seq_axs.dfy
@@ -1,0 +1,26 @@
+lemma LemmaTakeTake<T>()
+  ensures forall l: seq<T>, n, m: nat {:trigger l[..m][..n]} :: 0 <= n <= m <= |l| ==> (l[..m])[..n] == l[..n]
+{
+}
+lemma LemmaTakeAppend<T>()
+  ensures forall s, t: seq<T>, n: nat {:trigger (s+t)[..n]} :: 0 <= n <= |s| ==> (s+t)[..n] == s[..n]
+  ensures forall s, t: seq<T>, n: nat :: |s| <= n <= |s|+|t| ==> (s+t)[..n] == s + t[..n-|s|]
+{
+}
+lemma LemmaFullSlice<T>()
+  ensures forall s: seq<T> {:trigger s[..|s|]} :: s[..|s|] == s
+{
+}
+
+lemma LemmaEmptyAdd<T>()
+  ensures forall s, t: seq<T> :: t == [] ==> s + t == s && t + s == s
+{
+}
+
+lemma LemmaSequenceTheoryAuto<T>()
+  ensures forall l: seq<T>, n, m: nat {:trigger l[..m][..n]} :: 0 <= n <= m <= |l| ==> (l[..m])[..n] == l[..n]
+  ensures forall s, t: seq<T>, n: nat {:trigger (s+t)[..n]} :: 0 <= n <= |s| ==> (s+t)[..n] == s[..n]
+  ensures forall s, t: seq<T>, n: nat {:trigger (s+t)[..n]} :: |s| <= n <= |s|+|t| ==> (s+t)[..n] == s + t[..n-|s|]
+  ensures forall s: seq<T> {:trigger s[..|s|]} :: s[..|s|] == s
+  ensures forall s, t: seq<T> :: t == [] ==> s + t == s && t + s == s
+{}
